aarch64/CBuiltins.ml
@@ -17,16 +17,28 @@
 
 open C
 
-(* va_list is a struct of size 32 and alignment 8, passed by reference *)
+(* AAPCS64:
+     va_list is a struct of size 32 and alignment 8, passed by reference
+   Apple:
+     va_list is a pointer (size 8, alignment 8), passed by reference *)
 
-let va_list_type = TArray(TInt(IULong, []), Some 4L, [])
-let size_va_list = 32
-let va_list_scalar = false
+let (va_list_type, size_va_list, va_list_scalar) =
+  match Archi.abi with
+  | Archi.AAPCS64 -> (TArray(TInt(IULong, []), Some 4L, []), 32, false)
+  | Archi.Apple   -> (TPtr(TVoid [], []), 8, true)
+
+(* Some macOS headers use the GCC built-in types "__int128_t" and
+   "__uint128_t" unconditionally.  Provide a dummy definition. *)
+
+let int128_type = TArray(TInt(IULong, []), Some 2L, [])
 
 let builtins = {
-  builtin_typedefs = [
-    "__builtin_va_list", va_list_type
-  ];
+  builtin_typedefs =
+  [ "__builtin_va_list", va_list_type ] @
+  (if Configuration.system = "macosx" then
+  [ "__int128_t", int128_type;
+    "__uint128_t", int128_type ]
+  else []);
   builtin_functions = [
     (* Synchronization *)
     "__builtin_fence",
