aarch64/Archi.v
@@ -85,6 +85,10 @@ Global Opaque ptr64 big_endian splitlong
               fma_order fma_invalid_mul_is_nan
               float_of_single_preserves_sNaN.
 
-(** Whether to generate position-independent code or not *)
+(** Which ABI to implement *)
 
-Parameter pic_code: unit -> bool.
+Inductive abi_kind: Type :=
+  | AAPCS64 (**r ARM's standard as used in Linux and other ELF platforms *)
+  | Apple.  (**r the variant used in macOS and iOS *)
+
+Parameter abi: abi_kind.
